@prefix : <https://github.com/tibonto/Doc-BIAS/> .
@prefix mls: <http://www.w3.org/ns/mls#> .
@prefix owl: <http://www.w3.org/2002/07/owl#> .
@prefix rdf: <http://www.w3.org/1999/02/22-rdf-syntax-ns#> .
@prefix xml: <http://www.w3.org/XML/1998/namespace> .
@prefix xsd: <http://www.w3.org/2001/XMLSchema#> .
@prefix rdfs: <http://www.w3.org/2000/01/rdf-schema#> .
@prefix nobias: <https://github.com/tibonto/Doc-BIAS/> .
@base <https://github.com/tibonto/Doc-BIAS/> .

<https://github.com/tibonto/Doc-BIAS/> rdf:type owl:Ontology ;
                                        <http://purl.org/dc/elements/1.1/creator> "Maria-Esther Vidal"@en ,
                                                                                  "Mayra Russo"@en ,
                                                                                  "Yukti Sharma"@en ;
                                        rdfs:comment "An Ontology Design Pattern to Document Bias Events in Machine Learning Pipelines"@en .

#################################################################
#    Annotation properties
#################################################################

###  http://ontologydesignpatterns.org/opla-sd#entityPosition
<http://ontologydesignpatterns.org/opla-sd#entityPosition> rdf:type owl:AnnotationProperty .


###  http://ontologydesignpatterns.org/opla-sd#entityPositionX
<http://ontologydesignpatterns.org/opla-sd#entityPositionX> rdf:type owl:AnnotationProperty .


###  http://ontologydesignpatterns.org/opla-sd#entityPositionY
<http://ontologydesignpatterns.org/opla-sd#entityPositionY> rdf:type owl:AnnotationProperty .


###  http://purl.org/dc/elements/1.1/creator
<http://purl.org/dc/elements/1.1/creator> rdf:type owl:AnnotationProperty .


#################################################################
#    Object Properties
#################################################################

###  http://www.w3.org/ns/prov#wasGeneratedBy
<http://www.w3.org/ns/prov#wasGeneratedBy> rdf:type owl:ObjectProperty ;
                                           rdfs:subPropertyOf owl:topObjectProperty ;
                                           rdfs:domain nobias:Actor ;
                                           rdfs:range <http://www.w3.org/ns/prov#Activity> ;
                                           rdfs:comment "defines the provenance Activity that generates the Actor"@en ;
                                           rdfs:label "wasGeneratedBy"@en .


###  https://github.com/tibonto/Doc-BIAS/hasActorType
nobias:hasActorType rdf:type owl:ObjectProperty ;
                    rdfs:subPropertyOf owl:topObjectProperty ;
                    rdfs:domain nobias:Actor ;
                    rdfs:range nobias:ActorType ;
                    rdfs:comment "Describes Actor type: active or passive for Actor" .


###  https://github.com/tibonto/Doc-BIAS/hasBiasRecipient
nobias:hasBiasRecipient rdf:type owl:ObjectProperty ;
                        rdfs:subPropertyOf owl:topObjectProperty ;
                        owl:inverseOf nobias:hasBiasSource ;
                        rdfs:domain nobias:BiasSourceAgent ;
                        rdfs:range nobias:BiasRecipientAgent ;
                        rdfs:comment "Describes the relationship that has a bias recipient" .


###  https://github.com/tibonto/Doc-BIAS/hasBiasSource
nobias:hasBiasSource rdf:type owl:ObjectProperty ;
                     rdfs:subPropertyOf owl:topObjectProperty ;
                     rdfs:domain nobias:BiasRecipientAgent ;
                     rdfs:range nobias:BiasSourceAgent ;
                     rdfs:comment "Describes the relationship that has a bias source" .


###  https://github.com/tibonto/Doc-BIAS/hasBiasType
nobias:hasBiasType rdf:type owl:ObjectProperty ;
                   rdfs:subPropertyOf owl:topObjectProperty ;
                   rdf:type owl:FunctionalProperty ;
                   rdfs:domain nobias:BiasEvent ;
                   rdfs:range nobias:BiasType ;
                   rdfs:comment "describes the type of bias detected during the Bias Event" .


###  https://github.com/tibonto/Doc-BIAS/hasDetectionMethod
nobias:hasDetectionMethod rdf:type owl:ObjectProperty ;
                          rdfs:subPropertyOf owl:topObjectProperty ;
                          rdfs:domain nobias:BiasEvent ;
                          rdfs:range nobias:BiasDetectionMethod ;
                          rdfs:comment "describes the detection method for detecting bias during Bias Event" .


###  https://github.com/tibonto/Doc-BIAS/hasImplication
nobias:hasImplication rdf:type owl:ObjectProperty ;
                      rdfs:subPropertyOf owl:topObjectProperty ;
                      rdfs:domain nobias:BiasEvent ;
                      rdfs:range nobias:Implication ;
                      <http://purl.org/dc/elements/1.1/creator> "russo"^^xsd:string ;
                      rdfs:comment "Describes the relationship between implication and bias event."@en .


###  https://github.com/tibonto/Doc-BIAS/performsRecipientRole
nobias:performsRecipientRole rdf:type owl:ObjectProperty ;
                             rdfs:subPropertyOf owl:topObjectProperty ;
                             rdfs:domain nobias:BiasRecipientAgent ;
                             rdfs:range nobias:BiasRecipientRole ;
                             rdfs:comment "Describes the relationship that performs recipient role for the recipient agent" .


###  https://github.com/tibonto/Doc-BIAS/performsSourceRole
nobias:performsSourceRole rdf:type owl:ObjectProperty ;
                          rdfs:subPropertyOf owl:topObjectProperty ;
                          rdfs:domain nobias:BiasSourceAgent ;
                          rdfs:range nobias:BiasSourceRole ;
                          rdfs:comment "Describes the relationship that performs source role for the source agent" .


###  https://github.com/tibonto/Doc-BIAS/providesRecipientRole
nobias:providesRecipientRole rdf:type owl:ObjectProperty ;
                             rdfs:subPropertyOf owl:topObjectProperty ;
                             rdfs:domain nobias:BiasEvent ;
                             rdfs:range nobias:BiasRecipientRole ;
                             rdfs:comment "Describes the relationship that provides recipient role for the recipient agent" .


###  https://github.com/tibonto/Doc-BIAS/providesSourceRole
nobias:providesSourceRole rdf:type owl:ObjectProperty ;
                          rdfs:subPropertyOf owl:topObjectProperty ;
                          rdfs:domain nobias:BiasEvent ;
                          rdfs:range nobias:BiasSourceRole ;
                          rdfs:comment "Describes the relationship that provides source role for the source agent" .


###  https://github.com/tibonto/Doc-BIAS/subEventOf
nobias:subEventOf rdf:type owl:ObjectProperty ;
                  rdfs:subPropertyOf owl:topObjectProperty ;
                  rdf:type owl:ReflexiveProperty ;
                  rdfs:domain nobias:BiasEvent ;
                  rdfs:range nobias:BiasEvent ;
                  <http://purl.org/dc/elements/1.1/creator> "russo"^^xsd:string ;
                  rdfs:label "subEventOf"@en .


#################################################################
#    Data properties
#################################################################

###  https://github.com/tibonto/Doc-BIAS/hasBiasScore
nobias:hasBiasScore rdf:type owl:DatatypeProperty ;
                    rdfs:domain nobias:BiasEvent ;
                    rdfs:range xsd:decimal ;
                    rdfs:comment "Represents the bias score calculated with bias detection method" .


#################################################################
#    Classes
#################################################################

###  http://www.w3.org/ns/prov#Activity
<http://www.w3.org/ns/prov#Activity> rdf:type owl:Class ;
                                     rdfs:comment "This is an activity that provides provenance to the entities described in this pattern using a data source/dataset that is available and used for implementation of the Actor."@en ;
                                     rdfs:label "Activity"@en .


###  https://github.com/tibonto/Doc-BIAS/ActiveActor
nobias:ActiveActor rdf:type owl:Class ;
                   rdfs:subClassOf nobias:ActorType ;
                   <http://purl.org/dc/elements/1.1/creator> "russo"^^xsd:string ;
                   rdfs:label "ActiveActor"@en .


###  https://github.com/tibonto/Doc-BIAS/Actor
nobias:Actor rdf:type owl:Class ;
             rdfs:comment "Actors are identified elements of a particular domain. The interaction with other actors  is recorded as a bias event. They can influence bias, carry bias \"with\" themselves, and/or can also potentially propagate bias to other elements in the domain."@en ;
             rdfs:label "Actor"@en .


###  https://github.com/tibonto/Doc-BIAS/ActorType
nobias:ActorType rdf:type owl:Class ;
                 rdfs:comment "This is the type of relationship an actor has with bias. An active type of actor itself influences the bias while a passive type of actor can only carry bias from its source and itself has no influence on increasing or decreasing bias. It can only transfer bias." ;
                 rdfs:label "ActorType"@en .


###  https://github.com/tibonto/Doc-BIAS/BiasDetectionMethod
nobias:BiasDetectionMethod rdf:type owl:Class ;
                           rdfs:comment "The Class Bias Detection Method represents the method that was used to detect bias. For example, statistical analysis, expert assessment, quality metrics, etc."@en ;
                           rdfs:label "BiasDetectionMethod"@en .


###  https://github.com/tibonto/Doc-BIAS/BiasEvent
nobias:BiasEvent rdf:type owl:Class ;
                 rdfs:comment "A Bias Event is a class that represents an event entity that materializes when source and recipient participate and a detection method is identified. "@en ;
                 rdfs:label "BiasEvent"@en .


###  https://github.com/tibonto/Doc-BIAS/BiasRecipientAgent
nobias:BiasRecipientAgent rdf:type owl:Class ;
                          rdfs:comment "A Bias Recipient Agent acts as an agent between entities that provide a recipient role and the ones that are performing that role."@en ;
                          rdfs:label "BiasRecipientAgent"@en .


###  https://github.com/tibonto/Doc-BIAS/BiasRecipientRole
nobias:BiasRecipientRole rdf:type owl:Class ;
                         rdfs:comment "A Bias Recipien is the participant entity that participates as a recipient in a bias event."@en ;
                         rdfs:label "BiasRecipientRole"@en .


###  https://github.com/tibonto/Doc-BIAS/BiasSourceAgent
nobias:BiasSourceAgent rdf:type owl:Class ;
                       rdfs:comment "A Bias Source Agent acts as an agent between entities that provide the source role and the ones that are performing that role."@en ;
                       rdfs:label "BiasSourceAgent"@en .


###  https://github.com/tibonto/Doc-BIAS/BiasSourceRole
nobias:BiasSourceRole rdf:type owl:Class ;
                      rdfs:comment "A Bias Source is the participant entity that participates as a source in a bias event."@en ;
                      rdfs:label "BiasSourceRole"@en .


###  https://github.com/tibonto/Doc-BIAS/BiasType
nobias:BiasType rdf:type owl:Class ;
                rdfs:comment "This class represents the particular type of bias detected in a bias event. For example, it can be classified into social bias, behavioral bias, cognitive bias, functional bias, and statistical bias, among many other types of bias."@en ;
                rdfs:label "BiasType"@en .


###  https://github.com/tibonto/Doc-BIAS/EthicalImplication
nobias:EthicalImplication rdf:type owl:Class ;
                          rdfs:subClassOf nobias:Implication ;
                          <http://purl.org/dc/elements/1.1/creator> "russo"^^xsd:string ;
                          rdfs:comment "An ethical implication is an ethical consequence of a bias event. When evaluating this type of implication, moral considerations must be taken into account."@en ;
                          rdfs:label "EthicalImplication"@en .


###  https://github.com/tibonto/Doc-BIAS/Implication
nobias:Implication rdf:type owl:Class ;
                   rdfs:comment "Effects or consequences that  arise or may arise from the event taking place."@en ;
                   rdfs:label "Implication"@en .


###  https://github.com/tibonto/Doc-BIAS/Measurable
nobias:Measurable rdf:type owl:Class ;
                  rdfs:subClassOf nobias:BiasDetectionMethod ;
                  rdfs:comment "Measurable class defines the whether bias detection is measurable. For example, using quality/evaluation metrics." ;
                  rdfs:label "Measurable"@en .


###  https://github.com/tibonto/Doc-BIAS/NonMeasurable
nobias:NonMeasurable rdf:type owl:Class ;
                     rdfs:subClassOf nobias:BiasDetectionMethod ;
                     rdfs:comment "The NonMeasurable class represents a bias detection method that is not measurable. For example, cognitive biases." ;
                     rdfs:label "NonMeasurable"@en .


###  https://github.com/tibonto/Doc-BIAS/PassiveActor
nobias:PassiveActor rdf:type owl:Class ;
                    rdfs:subClassOf nobias:ActorType ;
                    <http://purl.org/dc/elements/1.1/creator> "russo"^^xsd:string ;
                    rdfs:label "PassiveActor"@en .


###  https://github.com/tibonto/Doc-BIAS/PracticalImplication
nobias:PracticalImplication rdf:type owl:Class ;
                            rdfs:subClassOf nobias:Implication ;
                            <http://purl.org/dc/elements/1.1/creator> "russo"^^xsd:string ;
                            rdfs:comment "A practical implication is the outcome or end result that occurs when a bias event takes place. Practical alludes to actual results that arise from the event."@en ;
                            rdfs:label "PracticalImplication"@en .


###  https://github.com/tibonto/Doc-BIAS/SocialImplication
nobias:SocialImplication rdf:type owl:Class ;
                         rdfs:subClassOf nobias:Implication ;
                         <http://purl.org/dc/elements/1.1/creator> "russo"^^xsd:string ;
                         rdfs:comment "A social implication refers to the effects a bias event has on such variables as the values, demographics, or economic condition of an individual or group of people."@en ;
                         rdfs:label "SocialImplication"@en .


[ <http://ontologydesignpatterns.org/opla-sd#entityPositionX> "177.80767233646273"^^xsd:double ;
  <http://ontologydesignpatterns.org/opla-sd#entityPositionY> "41.76693330457322"^^xsd:double ;
  rdfs:comment "This is an entity positioning annotation generated by CoModIDE (https://comodide.com/). Removing this annotation will break rendering the CoModIDE schema diagram view."@en
] .

[ <http://ontologydesignpatterns.org/opla-sd#entityPositionX> "25.724138437129156"^^xsd:double ;
   <http://ontologydesignpatterns.org/opla-sd#entityPositionY> "96.82085372645162"^^xsd:double ;
   rdfs:comment "This is an entity positioning annotation generated by CoModIDE (https://comodide.com/). Removing this annotation will break rendering the CoModIDE schema diagram view."@en
 ] .

[ <http://ontologydesignpatterns.org/opla-sd#entityPositionX> "158.58608500424603"^^xsd:double ;
   <http://ontologydesignpatterns.org/opla-sd#entityPositionY> "65.21112076038212"^^xsd:double ;
   rdfs:comment "This is an entity positioning annotation generated by CoModIDE (https://comodide.com/). Removing this annotation will break rendering the CoModIDE schema diagram view."@en
 ] .

[ <http://ontologydesignpatterns.org/opla-sd#entityPositionX> "204.99351592283745"^^xsd:double ;
   <http://ontologydesignpatterns.org/opla-sd#entityPositionY> "291.74078734960744"^^xsd:double ;
   rdfs:comment "This is an entity positioning annotation generated by CoModIDE (https://comodide.com/). Removing this annotation will break rendering the CoModIDE schema diagram view."@en
 ] .

[ <http://ontologydesignpatterns.org/opla-sd#entityPositionX> "190.69788013632754"^^xsd:double ;
   <http://ontologydesignpatterns.org/opla-sd#entityPositionY> "201.725096059717"^^xsd:double ;
   rdfs:comment "This is an entity positioning annotation generated by CoModIDE (https://comodide.com/). Removing this annotation will break rendering the CoModIDE schema diagram view."@en
 ] .

[ <http://ontologydesignpatterns.org/opla-sd#entityPositionX> "267.04297368899245"^^xsd:double ;
   <http://ontologydesignpatterns.org/opla-sd#entityPositionY> "235.0641941277196"^^xsd:double ;
   rdfs:comment "This is an entity positioning annotation generated by CoModIDE (https://comodide.com/). Removing this annotation will break rendering the CoModIDE schema diagram view."@en
 ] .

[ <http://ontologydesignpatterns.org/opla-sd#entityPositionX> "123.14507800623137"^^xsd:double ;
   <http://ontologydesignpatterns.org/opla-sd#entityPositionY> "108.21130233852331"^^xsd:double ;
   rdfs:comment "This is an entity positioning annotation generated by CoModIDE (https://comodide.com/). Removing this annotation will break rendering the CoModIDE schema diagram view."@en
 ] .

[ <http://ontologydesignpatterns.org/opla-sd#entityPositionX> "240.26759706965936"^^xsd:double ;
   <http://ontologydesignpatterns.org/opla-sd#entityPositionY> "205.65296633310575"^^xsd:double ;
   rdfs:comment "This is an entity positioning annotation generated by CoModIDE (https://comodide.com/). Removing this annotation will break rendering the CoModIDE schema diagram view."@en
 ] .

[ <http://ontologydesignpatterns.org/opla-sd#entityPositionX> "112.27942781635298"^^xsd:double ;
   <http://ontologydesignpatterns.org/opla-sd#entityPositionY> "222.30220118614724"^^xsd:double ;
   rdfs:comment "This is an entity positioning annotation generated by CoModIDE (https://comodide.com/). Removing this annotation will break rendering the CoModIDE schema diagram view."@en
 ] .

[ <http://ontologydesignpatterns.org/opla-sd#entityPositionX> "281.1950798190486"^^xsd:double ;
   <http://ontologydesignpatterns.org/opla-sd#entityPositionY> "21.379606640060185"^^xsd:double ;
   rdfs:comment "This is an entity positioning annotation generated by CoModIDE (https://comodide.com/). Removing this annotation will break rendering the CoModIDE schema diagram view."@en
 ] .

[ <http://ontologydesignpatterns.org/opla-sd#entityPositionX> "82.31268739888675"^^xsd:double ;
   <http://ontologydesignpatterns.org/opla-sd#entityPositionY> "56.076263521227254"^^xsd:double ;
   rdfs:comment "This is an entity positioning annotation generated by CoModIDE (https://comodide.com/). Removing this annotation will break rendering the CoModIDE schema diagram view."@en
 ] .

[ <http://ontologydesignpatterns.org/opla-sd#entityPositionX> "104.97298053840674"^^xsd:double ;
   <http://ontologydesignpatterns.org/opla-sd#entityPositionY> "18.62876625593159"^^xsd:double ;
   rdfs:comment "This is an entity positioning annotation generated by CoModIDE (https://comodide.com/). Removing this annotation will break rendering the CoModIDE schema diagram view."@en
 ] .

[ <http://ontologydesignpatterns.org/opla-sd#entityPositionX> "194.89241882997416"^^xsd:double ;
   <http://ontologydesignpatterns.org/opla-sd#entityPositionY> "78.5137806207522"^^xsd:double ;
   rdfs:comment "This is an entity positioning annotation generated by CoModIDE (https://comodide.com/). Removing this annotation will break rendering the CoModIDE schema diagram view."@en
 ] .

[ <http://ontologydesignpatterns.org/opla-sd#entityPositionX> "292.79187440316997"^^xsd:double ;
   <http://ontologydesignpatterns.org/opla-sd#entityPositionY> "215.92483065444162"^^xsd:double ;
   rdfs:comment "This is an entity positioning annotation generated by CoModIDE (https://comodide.com/). Removing this annotation will break rendering the CoModIDE schema diagram view."@en
 ] .

[ <http://ontologydesignpatterns.org/opla-sd#entityPositionX> "231.8286737721259"^^xsd:double ;
   <http://ontologydesignpatterns.org/opla-sd#entityPositionY> "63.091476370501134"^^xsd:double ;
   rdfs:comment "This is an entity positioning annotation generated by CoModIDE (https://comodide.com/). Removing this annotation will break rendering the CoModIDE schema diagram view."@en
 ] .

[ <http://ontologydesignpatterns.org/opla-sd#entityPositionX> "87.69248383502503"^^xsd:double ;
   <http://ontologydesignpatterns.org/opla-sd#entityPositionY> "47.05066588255914"^^xsd:double ;
   rdfs:comment "This is an entity positioning annotation generated by CoModIDE (https://comodide.com/). Removing this annotation will break rendering the CoModIDE schema diagram view."@en
 ] .

[ <http://ontologydesignpatterns.org/opla-sd#entityPositionX> "144.29573146880315"^^xsd:double ;
   <http://ontologydesignpatterns.org/opla-sd#entityPositionY> "37.353343225627306"^^xsd:double ;
   rdfs:comment "This is an entity positioning annotation generated by CoModIDE (https://comodide.com/). Removing this annotation will break rendering the CoModIDE schema diagram view."@en
 ] .

[ <http://ontologydesignpatterns.org/opla-sd#entityPositionX> "77.12635598660223"^^xsd:double ;
   <http://ontologydesignpatterns.org/opla-sd#entityPositionY> "16.515259324897947"^^xsd:double ;
   rdfs:comment "This is an entity positioning annotation generated by CoModIDE (https://comodide.com/). Removing this annotation will break rendering the CoModIDE schema diagram view."@en
 ] .

###  Generated by the OWL API (version 4.5.9.2019-02-01T07:24:44Z) https://github.com/owlcs/owlapi
